mailbox/verif_mailbox_all.v
@@ -14,30 +14,32 @@ Require Import mailbox.verif_mailbox_main.
 Section mpred.
 
 Context `{!VSTGS unit Σ, AEGS0 : !AEGS t_atom_int, !inG Σ (excl_authR (leibnizO val))}.
-Existing Instance concurrent_ext_spec.
+
+Definition ext_link := ext_link_prog prog.
+
+#[local] Instance AE_ext_spec : ext_spec unit := add_funspecs_rec unit ext_link (void_spec unit)
+  [(ext_link "make_atomic", SC_atomics.make_atomic_spec);
+   (ext_link "atom_exchange", SC_atomics.atomic_exchange_spec);
+   (ext_link "spawn", semax_conc.spawn_spec)].
 
 (* This lemma ties all the function proofs into a single proof for the entire program. *)
 Lemma all_funcs_correct:
-  semax_func Vprog Gprog (Genv.globalenv prog) (prog_funct prog) 
-   ltac:(old_with_library prog Gprog).
+  semax_prog prog tt Vprog Gprog.
 Proof.
-unfold prog, prog_funct, main_post, prog_vars; simpl.
-prove_semax_prog_setup_globalenv.
-repeat (eapply semax_func_cons_ext_vacuous; [reflexivity | reflexivity | LookupID | LookupB |]).
-repeat semax_func_cons_ext.
-semax_func_cons body_malloc. apply semax_func_cons_malloc_aux.
-repeat semax_func_cons_ext.
-{ unfold PROPx, LOCALx, SEPx, local, lift1, liftx, lift; simpl.
-  unfold liftx, lift; simpl.
-  Intros x; subst.
-  sep_apply lock_inv_isptr; Intros.
-  apply prop_right; unfold make_ext_rval, eval_id in *; simpl in *.
-  destruct ret; simpl in *; subst; auto. }
-{ unfold PROPx, LOCALx, SEPx, local, lift1, liftx, lift; simpl.
-  unfold liftx, lift; simpl.
-  Intros; subst.
-  apply prop_right; unfold make_ext_rval, eval_id in *; simpl in *.
-  destruct ret; simpl in *; subst; auto. }
+prove_semax_prog.
+semax_func_cons body_exit.
+semax_func_cons body_malloc.
+{ destruct x; apply semax_func_cons_malloc_aux. }
+semax_func_cons_ext.
+{ simpl; monPred.unseal; Intro p.
+  assert_PROP (isptr p); last by apply typecheck_return_value with (t := Tint16signed); auto.
+  rewrite /PROPx /LOCALx /SEPx; monPred.unseal.
+  rewrite !bi.and_elim_r.
+  rewrite bi.sep_emp; apply atomic_int_isptr. }
+semax_func_cons_ext.
+{ simpl; destruct x as ((((?, ?), ?), ?), ?); monPred.unseal; Intro i.
+  apply typecheck_return_value with (t := Tint16signed); auto. }
+semax_func_cons_ext.
 semax_func_cons body_surely_malloc.
 semax_func_cons body_memset.
 semax_func_cons body_initialize_channels.
@@ -45,10 +47,7 @@ semax_func_cons body_initialize_reader.
 semax_func_cons body_start_read.
 semax_func_cons body_finish_read.
 semax_func_cons body_initialize_writer.
-eapply semax_func_cons; [ reflexivity
-           | repeat apply Forall_cons; try apply Forall_nil; simpl; auto; computable
-           | unfold var_sizes_ok; repeat constructor; simpl; computable | reflexivity | LookupID | LookupB 
-           | apply body_start_write |].
+semax_func_cons body_start_write.
 semax_func_cons body_finish_write.
 semax_func_cons body_reader.
 semax_func_cons body_writer.
